src/Exp.v
@@ -3,6 +3,7 @@ Require Export
   Coq.Lists.List.
 
 From Equations Require Import Equations.
+Set Equations With UIP.
 
 Generalizable All Variables.
 
@@ -12,6 +13,7 @@ Import ListNotations.
 
 Class HostExprs (A : Type) : Type := {
   has_host_types :> HostTypes A;
+  HostErr : Type;
   HostExp : Ty → Type
 }.
 
@@ -23,32 +25,39 @@ Open Scope Ty_scope.
 Definition Env := list Ty.
 
 Inductive Var : Env → Ty → Type :=
-  | ZV Γ τ    : Var (τ :: Γ) τ
-  | SV Γ τ τ' : Var Γ τ → Var (τ' :: Γ) τ.
+  | ZV {Γ τ}    : Var (τ :: Γ) τ
+  | SV {Γ τ τ'} : Var Γ τ → Var (τ' :: Γ) τ.
 
 Derive Signature NoConfusion for Var.
 
+Inductive Err : Type :=
+  | CarOfNil
+  | HostedErr : HostErr → Err.
+
+Derive NoConfusion NoConfusionHom Subterm for Err.
+
 Inductive Exp Γ : Ty → Type :=
-  | HostedExp {τ}       : HostExp τ → Exp Γ τ
-  | HostedVal {ty}      : HostExp (TyHost ty) → Exp Γ (TyHost ty)
-  | HostedFun {dom cod} : HostExp (dom ⟶ cod) → Exp Γ (dom ⟶ cod)
+  (* | HostedExp {τ}       : HostExp τ → Exp Γ τ *)
+  (* | HostedVal {ty}      : HostExp (TyHost ty) → Exp Γ (TyHost ty) *)
+  (* | HostedFun {dom cod} : HostExp (dom ⟶ cod) → Exp Γ (dom ⟶ cod) *)
 
-  | EUnit               : Exp Γ TyUnit
-  | ETrue               : Exp Γ TyBool
-  | EFalse              : Exp Γ TyBool
-  | If {τ}              : Exp Γ TyBool → Exp Γ τ → Exp Γ τ → Exp Γ τ
+  (* | Error {τ}           : Err → Exp Γ τ *)
+  (* | EUnit               : Exp Γ TyUnit *)
+  (* | ETrue               : Exp Γ TyBool *)
+  (* | EFalse              : Exp Γ TyBool *)
+  (* | If {τ}              : Exp Γ TyBool → Exp Γ τ → Exp Γ τ → Exp Γ τ *)
 
-  | Pair {τ1 τ2}        : Exp Γ τ1 → Exp Γ τ2 → Exp Γ (TyPair τ1 τ2)
-  | Fst {τ1 τ2}         : Exp Γ (TyPair τ1 τ2) → Exp Γ τ1
-  | Snd {τ1 τ2}         : Exp Γ (TyPair τ1 τ2) → Exp Γ τ2
+  (* | Pair {τ1 τ2}        : Exp Γ τ1 → Exp Γ τ2 → Exp Γ (TyPair τ1 τ2) *)
+  (* | Fst {τ1 τ2}         : Exp Γ (TyPair τ1 τ2) → Exp Γ τ1 *)
+  (* | Snd {τ1 τ2}         : Exp Γ (TyPair τ1 τ2) → Exp Γ τ2 *)
 
-  | Nil {τ}             : Exp Γ (TyList τ)
-  | Cons {τ}            : Exp Γ τ → Exp Γ (TyList τ) → Exp Γ (TyList τ)
-  | Car {τ}             : Exp Γ τ → Exp Γ (TyList τ) → Exp Γ τ
-  | Cdr {τ}             : Exp Γ (TyList τ) → Exp Γ (TyList τ)
-  | IsNil {τ}           : Exp Γ (TyList τ) → Exp Γ TyBool
+  (* | Nil {τ}             : Exp Γ (TyList τ) *)
+  (* | Cons {τ}            : Exp Γ τ → Exp Γ (TyList τ) → Exp Γ (TyList τ) *)
+  (* | Car {τ}             : Exp Γ (TyList τ) → Exp Γ τ *)
+  (* | Cdr {τ}             : Exp Γ (TyList τ) → Exp Γ (TyList τ) *)
+  (* | IsNil {τ}           : Exp Γ (TyList τ) → Exp Γ TyBool *)
 
-  | Seq {τ τ'}          : Exp Γ τ' → Exp Γ τ → Exp Γ τ
+  (* | Seq {τ τ'}          : Exp Γ τ' → Exp Γ τ → Exp Γ τ *)
 
   (* These are the terms of the base lambda calculus *)
   | VAR {τ}             : Var Γ τ → Exp Γ τ
@@ -59,22 +68,23 @@ Derive Signature NoConfusionHom for Exp.
 
 Fixpoint Exp_size {Γ τ} (e : Exp Γ τ) : nat :=
   match e with
-  | HostedExp _ x => 1
-  | HostedVal _ x => 1
-  | HostedFun _ x => 1
-  | EUnit _       => 1
-  | ETrue _       => 1
-  | EFalse _      => 1
-  | If _ b t e    => 1 + Exp_size b + Exp_size t + Exp_size e
-  | Pair _ x y    => 1 + Exp_size x + Exp_size y
-  | Fst _ p       => 1 + Exp_size p
-  | Snd _ p       => 1 + Exp_size p
-  | Nil _         => 1
-  | Cons _ x xs   => 1 + Exp_size x + Exp_size xs
-  | Car _ d xs    => 1 + Exp_size d + Exp_size xs
-  | Cdr _ xs      => 1 + Exp_size xs
-  | IsNil _ xs    => 1 + Exp_size xs
-  | Seq _ x y     => 1 + Exp_size x + Exp_size y
+  (* | HostedExp _ x => 1 *)
+  (* | HostedVal _ x => 1 *)
+  (* | HostedFun _ x => 1 *)
+  (* | Error _ _     => 1 *)
+  (* | EUnit _       => 1 *)
+  (* | ETrue _       => 1 *)
+  (* | EFalse _      => 1 *)
+  (* | If _ b t e    => 1 + Exp_size b + Exp_size t + Exp_size e *)
+  (* | Pair _ x y    => 1 + Exp_size x + Exp_size y *)
+  (* | Fst _ p       => 1 + Exp_size p *)
+  (* | Snd _ p       => 1 + Exp_size p *)
+  (* | Nil _         => 1 *)
+  (* | Cons _ x xs   => 1 + Exp_size x + Exp_size xs *)
+  (* | Car _ xs      => 1 + Exp_size xs *)
+  (* | Cdr _ xs      => 1 + Exp_size xs *)
+  (* | IsNil _ xs    => 1 + Exp_size xs *)
+  (* | Seq _ x y     => 1 + Exp_size x + Exp_size y *)
   | VAR _ v       => 1
   | LAM _ e       => 1 + Exp_size e
   | APP _ e1 e2   => 1 + Exp_size e1 + Exp_size e2
@@ -86,28 +96,33 @@ Proof. repeat intro; subst; contradiction. Qed.
 
 End Exp.
 
-Arguments ZV {A H _ _}.
-Arguments SV {A H _ _ _} _.
+(* Arguments ZV {A H _ _}. *)
+(* Arguments SV {A H _ _ _} _. *)
 
-Arguments HostedExp {A H Γ τ} _.
-Arguments HostedVal {A H Γ ty} _.
-Arguments HostedFun {A H Γ dom cod} _.
-Arguments EUnit {A H Γ}.
-Arguments ETrue {A H Γ}.
-Arguments EFalse {A H Γ}.
-Arguments If {A H Γ τ} _ _ _.
-Arguments Pair {A H Γ τ1 τ2} _ _.
-Arguments Fst {A H Γ τ1 τ2} _.
-Arguments Snd {A H Γ τ1 τ2} _.
-Arguments Nil {A H Γ τ}.
-Arguments Cons {A H Γ τ} _ _.
-Arguments Car {A H Γ τ} _ _.
-Arguments Cdr {A H Γ τ} _.
-Arguments IsNil {A H Γ τ} _.
-Arguments Seq {A H Γ τ τ'} _ _.
-Arguments VAR {A H Γ τ} _.
-Arguments LAM {A H Γ dom cod} _.
-Arguments APP {A H Γ dom cod} _ _.
+(* Arguments HostedExp {A H Γ τ} _. *)
+(* Arguments HostedVal {A H Γ ty} _. *)
+(* Arguments HostedFun {A H Γ dom cod} _. *)
+(* Arguments Error {A H Γ τ} _. *)
+(* Arguments EUnit {A H Γ}. *)
+(* Arguments ETrue {A H Γ}. *)
+(* Arguments EFalse {A H Γ}. *)
+(* Arguments If {A H Γ τ} _ _ _. *)
+(* Arguments Pair {A H Γ τ1 τ2} _ _. *)
+(* Arguments Fst {A H Γ τ1 τ2} _. *)
+(* Arguments Snd {A H Γ τ1 τ2} _. *)
+(* Arguments Nil {A H Γ τ}. *)
+(* Arguments Cons {A H Γ τ} _ _. *)
+(* Arguments Car {A H Γ τ} _. *)
+(* Arguments Cdr {A H Γ τ} _. *)
+(* Arguments IsNil {A H Γ τ} _. *)
+(* Arguments Seq {A H Γ τ τ'} _ _. *)
+(* Arguments VAR {A H Γ τ} _. *)
+(* Arguments LAM {A H Γ dom cod} _. *)
+(* Arguments APP {A H Γ dom cod} _ _. *)
+
+Arguments VAR {Γ τ} _.
+Arguments LAM {Γ dom cod} _.
+Arguments APP {Γ dom cod} _ _.
 
 Notation "Γ ∋ τ" := (Var Γ τ) (at level 10).
 Notation "Γ ⊢ τ" := (Exp Γ τ) (at level 10).
