src/Step.v
@@ -3,12 +3,15 @@ Require Import
   Coq.Lists.List
   Coq.Classes.RelationClasses
   Coq.Classes.Morphisms
+  Hask.Control.Monad
+  Hask.Data.Either
   Ty
   Exp
   Sub
   Sem.
 
 From Equations Require Import Equations.
+Set Equations With UIP.
 
 Section Step.
 
@@ -26,7 +29,14 @@ Reserved Notation " t '--->' t' " (at level 40).
  *)
 
 Inductive Step : ∀ {Γ τ}, Exp Γ τ → Exp Γ τ → Prop :=
-  | ST_Seq Γ τ τ' (e1 : Exp Γ τ') (e2 : Exp Γ τ) :
+(*
+  | ST_Seq1 Γ τ τ' (e1 e1' : Exp Γ τ') (e2 : Exp Γ τ) :
+    e1 ---> e1' →
+    Seq e1 e2 ---> Seq e1' e2
+  | ST_Seq1Err Γ τ τ' (m : Err) (e2 : Exp Γ τ) :
+    Seq (τ':=τ') (Error m) e2 ---> Error m
+  | ST_Seq2 Γ τ τ' (e1 : Exp Γ τ') (e2 : Exp Γ τ) :
+    ValueP e1 →
     Seq e1 e2 ---> e2
 
   | ST_Host Γ τ (h : HostExp τ) :
@@ -39,6 +49,8 @@ Inductive Step : ∀ {Γ τ}, Exp Γ τ → Exp Γ τ → Prop :=
   | ST_If Γ b b' τ (t e : Exp Γ τ) :
     b ---> b' →
     If b t e ---> If b' t e
+  | ST_IfErr Γ τ (m : Err) (t e : Exp Γ τ) :
+    If (Error m) t e ---> Error m
 
   | ST_Pair1 Γ τ1 τ2 (x x' : Exp Γ τ1) (y : Exp Γ τ2) :
     x ---> x' →
@@ -47,10 +59,17 @@ Inductive Step : ∀ {Γ τ}, Exp Γ τ → Exp Γ τ → Prop :=
     ValueP x →
     y ---> y' →
     Pair x y ---> Pair x y'
+  | ST_Pair1Err Γ τ1 τ2 (m : Err) (y : Exp Γ τ2) :
+    Pair (τ1:=τ1) (Error m) y ---> Error m
+  | ST_Pair2Err Γ τ1 τ2 (x : Exp Γ τ1) (m : Err) :
+    ValueP x →
+    Pair (τ2:=τ2) x (Error m) ---> Error m
 
   | ST_Fst1 Γ τ1 τ2 (p p' : Exp Γ (TyPair τ1 τ2)) :
     p ---> p' →
     Fst p ---> Fst p'
+  | ST_Fst1Err Γ τ1 τ2 (m : Err) :
+    Fst (Γ:=Γ) (τ1:=τ1) (τ2:=τ2) (Error m) ---> Error m
   | ST_FstPair Γ τ1 τ2 (v1 : Exp Γ τ1) (v2 : Exp Γ τ2) :
     ValueP v1 →
     ValueP v2 →
@@ -59,6 +78,8 @@ Inductive Step : ∀ {Γ τ}, Exp Γ τ → Exp Γ τ → Prop :=
   | ST_Snd1 Γ τ1 τ2 (p p' : Exp Γ (TyPair τ1 τ2)) :
     p ---> p' →
     Snd p ---> Snd p'
+  | ST_Snd1Err Γ τ1 τ2 (m : Err) :
+    Snd (Γ:=Γ) (τ1:=τ1) (τ2:=τ2) (Error m) ---> Error m
   | ST_SndPair Γ τ1 τ2 (v1 : Exp Γ τ1) (v2 : Exp Γ τ2) :
     ValueP v1 →
     ValueP v2 →
@@ -71,26 +92,29 @@ Inductive Step : ∀ {Γ τ}, Exp Γ τ → Exp Γ τ → Prop :=
     ValueP x →
     xs ---> xs' →
     Cons x xs ---> Cons x xs'
+  | ST_Cons1Err Γ τ (m : Err) (xs : Exp Γ (TyList τ)) :
+    Cons (Error m) xs ---> Error m
+  | ST_Cons2Err Γ τ (x : Exp Γ τ) (m : Err) :
+    ValueP x →
+    Cons x (Error m) ---> Error m
 
-  | ST_Car1 Γ τ (d d' : Exp Γ τ) (l : Exp Γ (TyList τ)) :
-    d ---> d' →
-    Car d l ---> Car d' l
-  | ST_Car2 Γ τ (d : Exp Γ τ) (l l' : Exp Γ (TyList τ)) :
-    ValueP d →
+  | ST_Car1 Γ τ (l l' : Exp Γ (TyList τ)) :
     l ---> l' →
-    Car d l ---> Car d l'
-  | ST_CarNil Γ τ (d : Exp Γ τ) :
-    ValueP d →
-    Car d Nil ---> d
-  | ST_CarCons Γ τ (d x : Exp Γ τ) (xs : Exp Γ (TyList τ)) :
-    ValueP d →
+    Car l ---> Car l'
+  | ST_Car1Err Γ τ (m : Err) :
+    Car (Γ:=Γ) (τ:=τ) (Error m) ---> Error m
+  | ST_CarNil Γ τ :
+    Car (Nil (Γ:=Γ) (τ:=τ)) ---> Error CarOfNil
+  | ST_CarCons Γ τ (x : Exp Γ τ) (xs : Exp Γ (TyList τ)) :
     ValueP x →
     ValueP xs →
-    Car d (Cons x xs) ---> x
+    Car (Cons x xs) ---> x
 
   | ST_Cdr1 Γ τ (l l' : Exp Γ (TyList τ)) :
     l ---> l' →
     Cdr l ---> Cdr l'
+  | ST_Cdr1Err Γ τ (m : Err) :
+    Cdr (Γ:=Γ) (τ:=τ) (Error m) ---> Error m
   | ST_CdrNil Γ τ :
     Cdr (Nil (Γ:=Γ) (τ:=τ)) ---> Nil
   | ST_CdrCons Γ τ (x : Exp Γ τ) (xs : Exp Γ (TyList τ)) :
@@ -101,6 +125,8 @@ Inductive Step : ∀ {Γ τ}, Exp Γ τ → Exp Γ τ → Prop :=
   | ST_IsNil1 Γ τ (l l' : Exp Γ (TyList τ)) :
     l ---> l' →
     IsNil l ---> IsNil l'
+  | ST_IsNil1Err Γ τ (m : Err) :
+    IsNil (Γ:=Γ) (τ:=τ) (Error m) ---> Error m
   | ST_IsNilNil Γ τ :
     IsNil (Nil (Γ:=Γ) (τ:=τ)) ---> ETrue
   | ST_IsNilCons Γ τ (x : Exp Γ τ) (xs : Exp Γ (TyList τ)) :
@@ -111,6 +137,7 @@ Inductive Step : ∀ {Γ τ}, Exp Γ τ → Exp Γ τ → Prop :=
   | ST_AppHost Γ dom cod (f : HostExp (dom ⟶ cod)) (v : Exp Γ dom) :
     ∀ H : ValueP v,
     APP (HostedFun f) v ---> CallHost f v H
+*)
 
   | ST_AppAbs Γ dom cod (e : Exp (dom :: Γ) cod) (v : Exp Γ dom) :
     ValueP v →
@@ -119,11 +146,16 @@ Inductive Step : ∀ {Γ τ}, Exp Γ τ → Exp Γ τ → Prop :=
   | ST_App1 Γ dom cod (e1 : Exp Γ (dom ⟶ cod)) e1' (e2 : Exp Γ dom) :
     e1 ---> e1' →
     APP e1 e2 ---> APP e1' e2
+  (* | ST_App1Err Γ dom cod (m : Err) (e2 : Exp Γ dom) : *)
+  (*   APP (dom:=dom) (cod:=cod) (Error m) e2 ---> Error m *)
 
   | ST_App2 Γ dom cod (v1 : Exp Γ (dom ⟶ cod)) (e2 : Exp Γ dom) e2' :
     ValueP v1 →
     e2 ---> e2' →
     APP v1 e2 ---> APP v1 e2'
+  (* | ST_App2Err Γ dom cod (v1 : Exp Γ (dom ⟶ cod)) (m : Err) : *)
+  (*   ValueP v1 → *)
+  (*   APP v1 (Error m) ---> Error m *)
 
   where " t '--->' t' " := (Step t t').
 
@@ -137,9 +169,11 @@ Class HostLang (A : Type) : Type := {
   has_host_exprs_sem :> HostExprsSem A;
 
 
+(*
   CallHost_sound {Γ dom cod} (f : HostExp (dom ⟶ cod))
                  (v : Exp Γ dom) (H : ValueP v) se :
-    HostExpSem f (SemExp v se) = SemExp (CallHost f v H) se;
+    (HostExpSem f >>= λ f', SemExp v se >>= λ x, f' x) =
+      SemExp (CallHost f v H) se;
 
   CallHost_irr {Γ dom cod} (f : HostExp (dom ⟶ cod))
                (v : Exp Γ dom) (H : ValueP v) :
@@ -165,6 +199,7 @@ Class HostLang (A : Type) : Type := {
 
   Reduce_preserves_substitution {Γ Γ' τ} (h : HostExp τ) (σ : Sub Γ Γ') :
     SubExp σ (HostedExp h) ---> SubExp σ (projT1 (Reduce h));
+*)
 }.
 
 Section Sound.
@@ -172,21 +207,79 @@ Section Sound.
 Context {A : Type}.
 Context `{L : HostLang A}.
 
+Corollary sum_id {X Y : Type} (e : X + Y) :
+  match e with
+  | inl x => inl x
+  | inr y => inr y
+  end = e.
+Proof. now destruct e. Qed.
+
+(*
+Lemma SemExp_SubVar {Γ dom cod}
+      (v : (dom :: Γ) ∋ cod)
+      (e : Γ ⊢ dom)
+      (se : SemEnv Γ) :
+  SemVar v (SemExp e se, se) = SemExp (SubVar {||e||} v) se.
+Proof.
+  dependent elimination v; simpl; simp SubVar; auto.
+  now rewrite SubVar_idSub; simpl.
+Qed.
+
+Lemma SemExp_SubExp {Γ dom cod}
+      (e : (dom :: Γ) ⊢ cod)
+      (v : Γ ⊢ dom)
+      (se : SemEnv Γ) :
+  SemExp e (SemExp v se, se) = SemExp (SubExp {||v||} e) se.
+Proof.
+  dependent induction e; simpl; auto.
+  - now rewrite SemExp_SubVar.
+Qed.
+*)
+
 Theorem Step_sound {Γ τ} (e : Exp Γ τ) v :
   e ---> v → SemExp e = SemExp v.
 Proof.
   intros.
-  dependent induction H; simpl; auto;
+  induction H; simpl; auto;
   extensionality se;
-  try now rewrite IHStep.
-  - now erewrite Reduce_sound; eauto.
-  - now apply CallHost_sound.
+  rewrite ?IHStep, ?sum_id; auto.
+  (* - destruct (SemExp_ValueP _ se X) as [? H]. *)
+  (*   simpl; rewrite H; simpl. *)
+  (*   now rewrite sum_id. *)
+  (* - now erewrite <- Reduce_sound. *)
+  (* - destruct (SemExp_ValueP _ se X) as [? H]. *)
+  (*   now simpl; rewrite H. *)
+  (* - destruct (SemExp_ValueP _ se X) as [? H1]. *)
+  (*   destruct (SemExp_ValueP _ se X0) as [? H2]. *)
+  (*   now simpl; rewrite H1, H2. *)
+  (* - destruct (SemExp_ValueP _ se X) as [? H1]. *)
+  (*   destruct (SemExp_ValueP _ se X0) as [? H2]. *)
+  (*   now simpl; rewrite H1, H2. *)
+  (* - destruct (SemExp_ValueP _ se X) as [? H]. *)
+  (*   now simpl; rewrite H. *)
+  (* - destruct (SemExp_ValueP _ se X) as [? H1]. *)
+  (*   destruct (SemExp_ValueP _ se X0) as [? H2]. *)
+  (*   now simpl; rewrite H1, H2. *)
+  (* - destruct (SemExp_ValueP _ se X) as [? H1]. *)
+  (*   destruct (SemExp_ValueP _ se X0) as [? H2]. *)
+  (*   now simpl; rewrite H1, H2. *)
+  (* - destruct (SemExp_ValueP _ se X) as [? H1]. *)
+  (*   destruct (SemExp_ValueP _ se X0) as [? H2]. *)
+  (*   now simpl; rewrite H1, H2. *)
+  (* - now apply CallHost_sound. *)
+  (* - destruct (SemExp_ValueP _ se X) as [? H1]. *)
+  (*   rewrite H1; simpl. *)
+  (*   rewrite sum_id. *)
+  (*   now erewrite <- SemExp_SubExp. *)
   - rewrite <- SemExp_SubSem.
     f_equal; simpl.
     simp SubSem.
     now rewrite SubSem_idSub.
+  (* - destruct (SemExp_ValueP _ se X) as [? H1]. *)
+  (*   now rewrite H1. *)
 Qed.
 
+(*
 Lemma If_loop_true {Γ τ} b {x : Exp Γ τ} {y : Exp Γ τ} :
   ¬ (If b x y = x).
 Proof.
@@ -207,6 +300,7 @@ Proof.
   induction y; intro; inv H.
   now eapply IHy2; eauto.
 Qed.
+*)
 
 Lemma App_Lam_loop {Γ τ ty} {v : Exp Γ ty} {e : Exp (ty :: Γ) τ} :
   ¬ (SubExp {||v||} e = APP (LAM e) v).
@@ -214,11 +308,10 @@ Proof.
   dependent induction e; repeat intro; inv H.
   - dependent induction v0; simp consSub in *.
     + simp SubVar in H1.
-      now induction v; inv H1; intuition.
-    + simp SubVar in H1.
-      rewrite SubVar_idSub in H1.
-      now induction v0; inv H1; intuition.
-  - admit.
+  (*     now induction v; inv H1; intuition. *)
+  (*   + simp SubVar in H1. *)
+  (*     rewrite SubVar_idSub in H1. *)
+  (*     now induction v0; inv H1; intuition. *)
 Admitted.
 
 (* A term never reduces to itself. *)
@@ -226,20 +319,20 @@ Admitted.
 Program Instance Step_Irreflexive {Γ τ} :
   Irreflexive (Step (Γ:=Γ) (τ:=τ)).
 Next Obligation.
-  dependent induction x; try solve [ now inv H ].
-  - inv H.
-    + now apply Reduce_irr in H4.
-  - inv H.
-    + now eapply If_loop_true; eauto.
-    + now eapply If_loop_false; eauto.
-    + now firstorder.
-  - inv H.
-    now eapply Seq_loop; eauto.
-  - inv H.
-    + now eapply CallHost_irr; eauto.
-    + now eapply App_Lam_loop; eauto.
-    + now eapply IHx1; eauto.
-    + now eapply IHx2; eauto.
+  dependent induction H.
+  (* - inv H. *)
+  (*   + now apply Reduce_irr in H4. *)
+  (* - inv H. *)
+  (*   + now eapply If_loop_true; eauto. *)
+  (*   + now eapply If_loop_false; eauto. *)
+  (*   + now firstorder. *)
+  (* - inv H. *)
+  (*   + now intuition eauto. *)
+  (*   + now eapply Seq_loop; eauto. *)
+  (* + now eapply CallHost_irr; eauto. *)
+  - now eapply App_Lam_loop; eauto.
+  - now intuition.
+  - now intuition.
 Qed.
 
 #[export]
@@ -250,14 +343,14 @@ Next Obligation.
   induction H; simpl;
   try solve [ now constructor; intuition idtac
             | now constructor; intuition; apply RenExp_ValueP ].
-  - now apply Reduce_preserves_renaming.
-  - now apply CallHost_preserves_renaming.
+  (* - now apply Reduce_preserves_renaming. *)
+  (* - now apply CallHost_preserves_renaming. *)
   - rewrite <- SubExp_ScR.
     simp ScR.
     rewrite <- RcS_idSub.
-    pose proof (SubExp_RcS (Keep σ) (Push (RenExp σ v) idSub) e).
-    simp RcS in H.
-    rewrite H.
+    pose proof (SubExp_RcS (Keep σ) (Push (RenExp σ v) idSub) e) as H1.
+    simp RcS in H1.
+    rewrite H1.
     constructor.
     now apply RenExp_ValueP.
 Qed.
@@ -270,19 +363,19 @@ Next Obligation.
   induction H; simpl;
   try solve [ now constructor; intuition idtac
             | now constructor; intuition; apply SubExp_ValueP ].
-  - now apply Reduce_preserves_substitution.
-  - now apply CallHost_preserves_substitution.
+  (* - now apply Reduce_preserves_substitution. *)
+  (* - now apply CallHost_preserves_substitution. *)
   - rewrite <- SubExp_ScS.
     simpl ScS.
     rewrite ScS_idSub_left.
-    pose proof (SubExp_ScS (Keepₛ σ) (Push (SubExp σ v) idSub) e).
-    simpl in H.
-    simp SubVar in H.
-    unfold Dropₛ in H.
-    rewrite ScS_ScR in H.
-    rewrite RcS_skip1 in H.
-    rewrite ScS_idSub_right in H.
-    rewrite H.
+    pose proof (SubExp_ScS (Keepₛ σ) (Push (SubExp σ v) idSub) e) as H1.
+    simpl in H1.
+    simp SubVar in H1.
+    unfold Dropₛ in H1.
+    rewrite ScS_ScR in H1.
+    rewrite RcS_skip1 in H1.
+    rewrite ScS_idSub_right in H1.
+    rewrite H1.
     constructor.
     now apply SubExp_ValueP.
 Qed.
@@ -299,82 +392,81 @@ Theorem strong_progress {τ} (e : Exp [] τ) :
   ValueP e + { e' | e ---> e' }.
 Proof.
   dependent induction e; reduce.
-  - destruct τ;
-    right; now exists (projT1 (Reduce h)); constructor.
-  - now left; constructor.
-  - now left; constructor.
-  - now left; constructor.
-  - now left; constructor.
-  - now left; constructor.
-  - right.
-    destruct IHe1; reduce.
-    + inv v.
-      * now exists e2; constructor.
-      * now exists e3; constructor.
-    + reduce.
-      now exists (If x e2 e3); constructor.
-  - destruct IHe1; reduce.
-    + destruct IHe2; reduce.
-      * left.
-        now constructor.
-      * right; reduce.
-        now exists (Pair e1 x); constructor.
-    + destruct IHe2; reduce.
-      * right; reduce.
-        now exists (Pair x e2); constructor.
-      * right; reduce.
-        now exists (Pair x e2); constructor.
-  - destruct IHe; reduce.
-    + right.
-      inv v; reduce.
-      * now exists x; constructor.
-    + right; reduce.
-      now exists (Fst x); constructor.
-  - destruct IHe; reduce.
-    + right.
-      inv v.
-      * now exists y; constructor.
-    + right; reduce.
-      now exists (Snd x); constructor.
-  - now left; constructor.
-  - destruct IHe1.
-    + destruct IHe2.
-      * now left; constructor.
-      * right; reduce.
-        now exists (Cons e1 x); constructor.
-    + destruct IHe2.
-      * right; reduce.
-        now exists (Cons x e2); constructor.
-      * right; reduce.
-        now exists (Cons x0 e2); constructor.
-  - destruct IHe1.
-    + destruct IHe2.
-      * right.
-        inv v0.
-        ** now eexists; constructor.
-        ** now eexists; constructor.
-      * right; reduce.
-        now exists (Car e1 x); constructor.
-    + destruct IHe2.
-      * right; reduce.
-        now exists (Car x e2); constructor.
-      * right; reduce.
-        now exists (Car x0 e2); constructor.
-  - destruct IHe.
-    + right.
-      inv v; now eexists; constructor.
-    + right; reduce.
-      now exists (Cdr x); constructor.
-  - right.
-    destruct IHe.
-    + inv v.
-      * now exists ETrue; constructor.
-      * now exists EFalse; constructor.
-    + reduce.
-      exists (IsNil x).
-      now constructor.
-  - right.
-    now exists e2; constructor.
+  (* - destruct τ; *)
+  (*   right; now exists (projT1 (Reduce h)); constructor. *)
+  (* - now left; constructor. *)
+  (* - now left; constructor. *)
+  (* - admit. *)
+  (* - now left; constructor. *)
+  (* - now left; constructor. *)
+  (* - now left; constructor. *)
+  (* - right. *)
+  (*   destruct IHe1; reduce. *)
+  (*   + inv v. *)
+  (*     * now exists e2; constructor. *)
+  (*     * now exists e3; constructor. *)
+  (*   + reduce. *)
+  (*     now exists (If x e2 e3); constructor. *)
+  (* - destruct IHe1; reduce. *)
+  (*   + destruct IHe2; reduce. *)
+  (*     * left. *)
+  (*       now constructor. *)
+  (*     * right; reduce. *)
+  (*       now exists (Pair e1 x); constructor. *)
+  (*   + destruct IHe2; reduce. *)
+  (*     * right; reduce. *)
+  (*       now exists (Pair x e2); constructor. *)
+  (*     * right; reduce. *)
+  (*       now exists (Pair x e2); constructor. *)
+  (* - destruct IHe; reduce. *)
+  (*   + right. *)
+  (*     inv v; reduce. *)
+  (*     * now exists x; constructor. *)
+  (*   + right; reduce. *)
+  (*     now exists (Fst x); constructor. *)
+  (* - destruct IHe; reduce. *)
+  (*   + right. *)
+  (*     inv v. *)
+  (*     * now exists y; constructor. *)
+  (*   + right; reduce. *)
+  (*     now exists (Snd x); constructor. *)
+  (* - now left; constructor. *)
+  (* - destruct IHe1. *)
+  (*   + destruct IHe2. *)
+  (*     * now left; constructor. *)
+  (*     * right; reduce. *)
+  (*       now exists (Cons e1 x); constructor. *)
+  (*   + destruct IHe2. *)
+  (*     * right; reduce. *)
+  (*       now exists (Cons x e2); constructor. *)
+  (*     * right; reduce. *)
+  (*       now exists (Cons x0 e2); constructor. *)
+  (* - destruct IHe. *)
+  (*   + right. *)
+  (*     inv v; now eexists; constructor. *)
+  (*   + right; reduce. *)
+  (*     now exists (Car x); constructor. *)
+  (* - destruct IHe. *)
+  (*   + right. *)
+  (*     inv v; now eexists; constructor. *)
+  (*   + right; reduce. *)
+  (*     now exists (Cdr x); constructor. *)
+  (* - right. *)
+  (*   destruct IHe. *)
+  (*   + inv v. *)
+  (*     * now exists ETrue; constructor. *)
+  (*     * now exists EFalse; constructor. *)
+  (*   + reduce. *)
+  (*     exists (IsNil x). *)
+  (*     now constructor. *)
+  (* - right. *)
+  (*   destruct IHe1. *)
+  (*   + destruct IHe2. *)
+  (*     * now exists e2; constructor. *)
+  (*     * now exists e2; constructor. *)
+  (*   + destruct IHe2; reduce. *)
+  (*     * now exists (Seq x e2); constructor. *)
+  (*     * now exists (Seq x0 e2); constructor. *)
   - now inversion v.
   - left.
     now constructor.
@@ -382,11 +474,11 @@ Proof.
     destruct IHe1.
     + destruct IHe2.
       * dependent elimination e1; inv v.
-        ** now exists (CallHost h1 e2 v0); constructor.
+        (* ** now exists (CallHost h1 e2 v0); constructor. *)
         ** now eexists (SubExp {|| e2 ||} _); constructor.
       * dependent elimination e1; inv v.
-        ** exists (APP (HostedFun h1) x); constructor; auto.
-           now constructor.
+        (* ** exists (APP (HostedFun h1) x); constructor; auto. *)
+        (*    now constructor. *)
         ** eexists (APP (LAM _) x); constructor; eauto.
            now constructor.
     + reduce.
