src/Value.v
@@ -3,6 +3,7 @@ Require Export
   Exp.
 
 From Equations Require Import Equations.
+Set Equations With UIP.
 
 Generalizable All Variables.
 
@@ -18,16 +19,17 @@ Open Scope Ty_scope.
 (* [ValueP] is an inductive proposition that indicates whether an expression
    represents a value, i.e., that it does reduce any further. *)
 Inductive ValueP Γ : ∀ {τ}, Exp Γ τ → Type :=
-  | HostedValP {ty} (x : HostExp (TyHost ty)) : ValueP Γ (HostedVal x)
-  | HostedFunP {dom cod} (f : HostExp (dom ⟶ cod)) : ValueP Γ (HostedFun f)
-  | UnitP : ValueP Γ EUnit
-  | TrueP : ValueP Γ ETrue
-  | FalseP : ValueP Γ EFalse
-  | PairP {τ1 τ2} {x : Exp Γ τ1} {y : Exp Γ τ2} :
-    ValueP Γ x → ValueP Γ y → ValueP Γ (Pair x y)
-  | NilP {τ} : ValueP Γ (Nil (τ:=τ))
-  | ConsP {τ} (x : Exp Γ τ) xs :
-    ValueP Γ x → ValueP Γ xs → ValueP Γ (Cons x xs)
+  (* | HostedValP {ty} (x : HostExp (TyHost ty)) : ValueP Γ (HostedVal x) *)
+  (* | HostedFunP {dom cod} (f : HostExp (dom ⟶ cod)) : ValueP Γ (HostedFun f) *)
+  (* | ErrorP {τ} m : ValueP Γ (Error (τ:=τ) m) *)
+  (* | UnitP        : ValueP Γ EUnit *)
+  (* | TrueP        : ValueP Γ ETrue *)
+  (* | FalseP       : ValueP Γ EFalse *)
+  (* | PairP {τ1 τ2} {x : Exp Γ τ1} {y : Exp Γ τ2} : *)
+  (*   ValueP Γ x → ValueP Γ y → ValueP Γ (Pair x y) *)
+  (* | NilP {τ} : ValueP Γ (Nil (τ:=τ)) *)
+  (* | ConsP {τ} (x : Exp Γ τ) xs : *)
+  (*   ValueP Γ x → ValueP Γ xs → ValueP Γ (Cons x xs) *)
   | LambdaP {dom cod} (e : Exp (dom :: Γ) cod) : ValueP Γ (LAM e).
 
 Derive Signature NoConfusion NoConfusionHom for ValueP.
@@ -36,23 +38,25 @@ Lemma ValueP_irrelevance {Γ τ} (v : Exp Γ τ) (H1 H2 : ValueP _ v) :
   H1 = H2.
 Proof.
   induction H1; dependent elimination H2; auto.
-  - now erewrite IHValueP1, IHValueP2; eauto.
-  - now erewrite IHValueP1, IHValueP2; eauto.
+  (* - now erewrite IHValueP1, IHValueP2; eauto. *)
+  (* - now erewrite IHValueP1, IHValueP2; eauto. *)
 Qed.
 
 Inductive Value : Ty → Type :=
-  | HostValue {ty}         : HostExp (TyHost ty) → Value (TyHost ty)
-  | VUnit                  : Value TyUnit
-  | VTrue                  : Value TyBool
-  | VFalse                 : Value TyBool
-  | VPair {τ1 τ2}          : Value τ1 → Value τ2 → Value (TyPair τ1 τ2)
-  | VNil {τ}               : Value (TyList τ)
-  | VCons {τ}              : Value τ → Value (TyList τ) → Value (TyList τ)
+  (* | HostValue {ty}         : HostExp (TyHost ty) → Value (TyHost ty) *)
+  (* | VError {τ} (m : Err)   : Value τ *)
+  (* | VUnit                  : Value TyUnit *)
+  (* | VTrue                  : Value TyBool *)
+  (* | VFalse                 : Value TyBool *)
+  (* | VPair {τ1 τ2}          : Value τ1 → Value τ2 → Value (TyPair τ1 τ2) *)
+  (* | VNil {τ}               : Value (TyList τ) *)
+  (* | VCons {τ}              : Value τ → Value (TyList τ) → Value (TyList τ) *)
   | ClosureExp {dom cod}   : Closure dom cod → Value (dom ⟶ cod)
 
 with Closure : Ty → Ty → Type :=
   | Lambda {dom cod}   : Exp [dom] cod → Closure dom cod
-  | Func {dom cod}     : HostExp (dom ⟶ cod) → Closure dom cod.
+  (* | Func {dom cod}     : HostExp (dom ⟶ cod) → Closure dom cod *)
+.
 
 Derive Signature NoConfusion NoConfusionHom for Value.
 Derive Signature NoConfusion NoConfusionHom Subterm for Closure.
@@ -69,12 +73,16 @@ Equations get_value `(s : ValEnv Γ) `(v : Var Γ τ) : Value τ :=
 
 End Value.
 
-Arguments ValueP {A H Γ τ} _.
-Arguments HostedValP {A H Γ ty} _.
-Arguments HostedFunP {A H Γ dom cod} _.
-Arguments TrueP {A H Γ}.
-Arguments FalseP {A H Γ}.
-Arguments PairP {A H Γ τ1 τ2 x y} _ _.
-Arguments NilP {A H Γ τ}.
-Arguments ConsP {A H Γ τ _ _} _ _.
-Arguments LambdaP {A H Γ dom cod} _.
+(* Arguments ValueP {A H Γ τ} _. *)
+(* Arguments HostedValP {A H Γ ty} _. *)
+(* Arguments HostedFunP {A H Γ dom cod} _. *)
+(* Arguments ErrorP {A H Γ τ} _. *)
+(* Arguments TrueP {A H Γ}. *)
+(* Arguments FalseP {A H Γ}. *)
+(* Arguments PairP {A H Γ τ1 τ2 x y} _ _. *)
+(* Arguments NilP {A H Γ τ}. *)
+(* Arguments ConsP {A H Γ τ _ _} _ _. *)
+(* Arguments LambdaP {A H Γ dom cod} _. *)
+
+Arguments ValueP {Γ τ} _.
+Arguments LambdaP {Γ dom cod} _.
