src/Ctxt.v
@@ -1,0 +1,69 @@
+Require Export
+  Ty
+  Coq.Lists.List
+  Exp
+  Sub.
+
+From Equations Require Import Equations.
+Set Equations With UIP.
+
+Generalizable All Variables.
+
+(** Evaluation contexts *)
+
+Section Ctxt.
+
+Import ListNotations.
+
+Context {A : Type}.
+Context `{HostExprs A}.
+
+Open Scope Ty_scope.
+
+Inductive Ctxt Γ : Ty → Type :=
+  | C_Hole {τ} : Ctxt Γ τ
+
+  (* | C_If1 {τ} : Ctxt Γ TyBool → Exp Γ τ → Exp Γ τ → Ctxt Γ TyBool *)
+  (* | C_If2 {τ} : Exp Γ TyBool → Ctxt Γ τ → Exp Γ τ → Ctxt Γ τ *)
+  (* | C_If3 {τ} : Exp Γ TyBool → Exp Γ τ → Ctxt Γ τ → Ctxt Γ τ *)
+
+  | C_App1 {dom cod} : Ctxt Γ (dom ⟶ cod) -> Exp Γ dom -> Ctxt Γ (dom ⟶ cod)
+  | C_App2 {dom cod} : Exp Γ (dom ⟶ cod) -> Ctxt Γ dom -> Ctxt Γ dom.
+
+Derive Signature NoConfusion NoConfusionHom for Ctxt.
+
+Inductive Plug : ∀ {Γ τ τ'}, Ctxt Γ τ → Exp Γ τ → Exp Γ τ' → Prop :=
+  | Plug_Hole {Γ τ} (e : Exp Γ τ) : Plug (C_Hole _) e e
+
+  (* | Plug_If1 {Γ τ} (C : Ctxt Γ TyBool) (e e' : Exp Γ TyBool) (e1 e2 : Exp Γ τ) : *)
+  (*   Plug C e e' -> Plug (C_If1 _ C e1 e2) e (If e' e1 e2) *)
+  (* | Plug_If2 {Γ τ} (C : Ctxt Γ τ) (e e' : Exp Γ τ) e1 (e2 : Exp Γ τ) : *)
+  (*   Plug C e e' -> Plug (C_If2 _ e1 C e2) e (If e1 e' e2) *)
+  (* | Plug_If3 {Γ τ} (C : Ctxt Γ τ) (e e' : Exp Γ τ) e1 (e2 : Exp Γ τ) : *)
+  (*   Plug C e e' -> Plug (C_If3 _ e1 e2 C) e (If e1 e2 e') *)
+
+  | Plug_App1 {Γ dom cod} (C : Ctxt Γ (dom ⟶ cod)) (e e' : Exp Γ (dom ⟶ cod))
+              (e1 : Exp Γ dom) :
+    Plug C e e' -> Plug (C_App1 _ C e1) e (APP e' e1)
+  | Plug_App2 {Γ dom cod} (C : Ctxt Γ dom) (e e' : Exp Γ dom)
+              (e1 : Exp Γ (dom ⟶ cod)) :
+    Plug C e e' -> Plug (C_App2 _ e1 C) e (APP e1 e').
+
+Derive Signature for Plug.
+
+Inductive Step0 : ∀ {Γ τ}, Exp Γ τ -> Exp Γ τ -> Prop :=
+  | ST_AppAbs0 {Γ dom cod} (e : Exp (dom :: Γ) cod) v :
+    ValueP v -> Step0 (APP (LAM e) v) (SubExp {|| v ||} e).
+
+Derive Signature for Step0.
+
+Inductive Step : ∀ {Γ τ}, Exp Γ τ -> Exp Γ τ -> Prop :=
+  | StepRule {Γ τ} (C : Ctxt Γ τ) (e1 e1' e2 e2' : Exp Γ τ) :
+    Plug C e1 e1' ->
+    Plug C e2 e2' ->
+    Step0 e1 e2 ->
+    Step e1' e2'.
+
+Derive Signature for Step.
+
+End Ctxt.
