src/Log.v
@@ -8,6 +8,7 @@ Require Import
   Sub.
 
 From Equations Require Import Equations.
+Set Equations With UIP.
 
 Generalizable All Variables.
 
