src/ilist.v
@@ -3,6 +3,7 @@ Require Import
   Coq.Lists.List.
 
 From Equations Require Import Equations.
+Set Equations With UIP.
 
 Generalizable All Variables.
 
