default.nix
@@ -11,6 +11,15 @@ args@{
 
 let
 
+inherit
+  (pkgs.callPackages
+    (pkgs.fetchFromGitHub {
+      owner = "jwiegley";
+      repo = "coq-haskell";
+      rev = "c46434df74e0de8c398b55cce30e6a764916e9e7";
+      sha256 = "01rd8zlgwb24lwxlzrb85zs3qzl6hp1ig88zv5a5g4b6pch0fliy";
+    }) {}) coq-haskell;
+
 pact-model = coqPackages: with pkgs.${coqPackages}; pkgs.stdenv.mkDerivation rec {
   name = "coq${coq.coq-version}-pact-model-${version}";
   version = "1.0";
@@ -20,8 +29,9 @@ pact-model = coqPackages: with pkgs.${coqPackages}; pkgs.stdenv.mkDerivation rec
         else ./.;
 
   buildInputs = [
-    coq coq.ocaml coq.camlp5 coq.findlib equations category-theory
-    # coqhammer pkgs.z3-tptp
+    coq coq.ocaml coq.camlp5 coq.findlib
+    equations category-theory (coq-haskell coqPackages)
+    coqhammer pkgs.z3-tptp
   ];
   enableParallelBuilding = true;
 
